pulse/lib/pulse/core/PulseCore.Atomic.fst
@@ -237,6 +237,9 @@ let with_invariant
 : stt_atomic a #obs (add_inv f_opens i) fp fp'
 = A.with_invariant i f
 
+let distinct_invariants_have_distinct_names = A.distinct_invariants_have_distinct_names
+let invariant_name_identifies_invariant = A.invariant_name_identifies_invariant
+
 let pts_to_not_null #a #p r v = Ghost.hide (A.pts_to_not_null #a #p r v)
 let alloc = A.alloc
 let read = A.read
