pulse/lib/pulse/lib/Pulse.Lib.Core.fsti
@@ -359,6 +359,26 @@ val with_invariant
                             (fun x -> p ** fp' x))
 : stt_atomic a #(join_obs obs Unobservable) (add_inv f_opens i) fp fp'
 
+val distinct_invariants_have_distinct_names
+    (#p #q:vprop)
+    (i:inv p)
+    (j:inv q { (p =!= q) })
+: stt_atomic (_:squash (name_of_inv i =!= name_of_inv j))
+    #Unobservable
+    emp_inames
+    emp
+    (fun _ -> emp)
+
+val invariant_name_identifies_invariant
+      (#p #q:vprop)
+      (i:inv p)
+      (j:inv q { name_of_inv i == name_of_inv j } )
+: stt_atomic (squash (p == q /\ i == j))
+    #Unobservable
+    emp_inames
+    emp
+    (fun _ -> emp)
+
 //////////////////////////////////////////////////////////////////////////
 // Ghost computations
 //////////////////////////////////////////////////////////////////////////
